\documentclass[a4paper]{article}
\usepackage[
	top=1in,
	bottom=1.75in,
	left=1.25in,
	right=1.25in
]{geometry}
\usepackage{algorithm}
\usepackage{amsmath}
\usepackage{algpseudocode}
\usepackage{pdfpages}
\usepackage{amssymb}
\usepackage{qtree}
\newcommand\qlabelhook{\it}
\usepackage{graphicx}
\usepackage{caption}
\usepackage{subcaption}

\def\sizeablebox[#1,#2,#3]{
		\hbox to #2 {\framebox[#1]{#3}}%
	}
\def\qframesubtree{\setbox\treeboxone \hbox{\framebox[1\width]{\box\treeboxone}}}

\usepackage[UKenglish]{babel}% http://ctan.org/pkg/babel
\usepackage[UKenglish]{isodate}% http://ctan.org/pkg/isodate
\cleanlookdateon

\begin{document}
	\title{Workshop Week 3}
	\author{Christian Nassif-Haynes}
	\maketitle

	\setcounter{section}{2}
	\section{Grammar Derivations And Parse Trees}
	Derivation and parse tree for \verb=(a,b)=:
	\begin{figure}[h]
		\centering
		\begin{subfigure}{0.48\textwidth}
			\centering
			\begin{align*}
				P &\rightarrow S & \\
				  &\rightarrow \text{ ( } L \text{ ) } & (2) \\
				  &\rightarrow \text{ ( } L \text{ , } S \text{ ) } & (3) \\
				  &\rightarrow \text{ ( } S \text{ , } S \text{ ) } & (3) \\
				  &\rightarrow \text{ ( a , } S \text{ ) } & (2) \\
				  &\rightarrow \text{ ( a , a ) } & (2)
			\end{align*}
		\end{subfigure}
		\begin{subfigure}{0.48\textwidth}
			\centering
			\Tree[.P
					[.S
						[ ( ]
						[.L
							[.L
								[.S
									a ]]
							[ , ]
							[.S
								a ]]
						[ ) ]]]
		\end{subfigure}
	\end{figure}
	
	Derivation and parse tree for \verb=(a,(a,a))=:
	\begin{figure}[h]
		\centering
		\begin{subfigure}{0.48\textwidth}
			\centering
			\begin{align*}
				P &\rightarrow S & \\
				  &\rightarrow \text{ ( } L \text{ ) } & (2) \\
				  &\rightarrow \text{ ( } L \text{ , } S \text{ ) } & (3) \\
				  &\rightarrow \text{ ( } S \text{ , } S \text{ ) } & (3) \\
				  &\rightarrow \text{ ( a , } S \text{ ) } & (2) \\
				  &\rightarrow \text{ ( a , ( } L \text{ ) ) } & (2) \\
				  &\rightarrow \text{ ( a , ( } L \text{ , } S \text{ ) ) } & (3) \\
				  &\rightarrow \text{ ( a , ( } S \text{ , } S \text{ ) ) } & (3) \\
				  &\rightarrow \text{ ( a , ( a , } S \text{ ) ) } & (2) \\
				  &\rightarrow \text{ ( a , ( a , a ) ) } & (2)
			\end{align*}
		\end{subfigure}
		\begin{subfigure}{0.50\textwidth}
			\centering
			\Tree[.P
					[.S
						[ ( ]
						[.L
							[.L
								[.S
									a ]]
							[ , ]
							[.S
								[ ( ]
								[.L
									[.L
										[.S
											a ]]
									[ , ]
									[.S
										a ]]
								[ ) ]]]
						[ ) ]]!{\qframesubtree} ]
		\end{subfigure}
	\end{figure}
	
	Derivation and parse tree for \verb=((a,(a,a)),a)= is show below. The triangle represents the framed section of the parse tree from the previous answer:
	\begin{figure}[h]
		\centering
		\begin{subfigure}{0.48\textwidth}
			\centering
			\begin{align*}
				P &\rightarrow S & \\
				  &\rightarrow \text{ ( } L \text{ ) } & (2) \\
				  &\rightarrow \text{ ( } L \text{ , } S \text{ ) } & (3) \\
				  &\rightarrow \text{ ( } S \text{ , } S \text{ ) } & (3) \\
				  &\rightarrow \text{ ( ( } L \text{ ) , } S \text{ ) } & (2) \\
				  &\rightarrow \text{ ( ( } L \text{ , } S \text{ ) , } S \text{ ) } & (3) \\
				  &\rightarrow \text{ ( ( } S \text{ , } S \text{ ) , } S \text{ ) } & (3) \\
				  &\rightarrow \text{ ( ( a , } S \text{ ) , } S \text{ ) } & (2) \\
				  &\rightarrow \text{ ( ( a , ( } L \text{ ) ) , } S \text{ ) } & (2) \\
				  &\rightarrow \text{ ( ( a , ( } L \text{ , } S \text{ ) ) , } S \text{ ) } & (3) \\
				  &\rightarrow \text{ ( ( a , ( } S \text{ , } S \text{ ) ) , } S \text{ ) } & (3) \\
				  &\rightarrow \text{ ( ( a , ( a , } S \text{ ) ) , } S \text{ ) } & (2) \\
				  &\rightarrow \text{ ( ( a , ( a , a ) ) , } S \text{ ) } & (2) \\
				  &\rightarrow \text{ ( ( a , ( a , a ) ) , a ) } & (2)
			\end{align*}
		\end{subfigure}
		\begin{subfigure}{0.48\textwidth}
			\centering
			\Tree[.P
					[.S
						[ ( ]
						[.L
							[.L \qroof{(a,(a,a))}.S ]
							[ , ]
							[.S
								a ]]
						[ ) ]]]
				\end{subfigure}
	\end{figure}
	
	\section{Ambiguous Grammars}
	The string \verb=abab= has precisely two parses under the given grammar:
	%{[}{]}
	\begin{itemize}
		\item {[}P {[}S a {[}S $\epsilon${]} b {[}S a {[}S $\epsilon${]} b {[}S $\epsilon${]}{]}{]}{]}
		\item {[}P {[}S a {[}S b {[}S $\epsilon${]} a {[}S $\epsilon${]}{]} b {[}S $\epsilon${]}{]}{]}
	\end{itemize}
\end{document}
